thys/Superposition_Calculus/Infinite_Variables_Per_Type.thy
@@ -1,0 +1,14 @@
+theory Infinite_Variables_Per_Type
+  imports Fun_Extra Fresh_Identifiers.Fresh
+begin
+
+definition infinite_variables_per_type where 
+  "infinite_variables_per_type \<V> \<equiv> \<forall>ty. infinite {x. \<V> x = ty}"
+
+lemma exists_infinite_variables_per_type:
+  assumes "|UNIV :: 'ty set| \<le>o |UNIV :: ('v :: infinite) set|"
+  shows "\<exists>\<V> :: ('v :: infinite \<Rightarrow> 'ty). infinite_variables_per_type \<V>"
+  using infinite_domain[OF assms infinite_UNIV]
+  unfolding infinite_variables_per_type_def.
+
+end
