thys/Superposition_Calculus/Nonground_Term_Typing.thy
@@ -219,33 +219,22 @@ next
   then show "welltyped \<V>' t \<tau>"
     by (induction rule: welltyped.induct) (simp_all add: welltyped.simps list.rel_mono_strong)
 next
-  fix \<V> \<V>' :: "('v, 'ty) var_types" and t :: "('f, 'v) term" and \<rho> \<tau> 
-  assume renaming: "term_subst.is_renaming \<rho>" "\<forall>x\<in>term.vars (t \<cdot>t \<rho>). \<V> (inv \<rho> (Var x)) = \<V>' x"
+  fix \<V> \<V>' :: "('v, 'ty) var_types" and t :: "('f, 'v) term" and \<rho> :: "('f, 'v) subst" and \<tau> 
+  assume renaming: "term_subst.is_renaming \<rho>" and \<V>: "\<forall>x\<in>term.vars t. \<V> x = \<V>' (term.rename \<rho> x)"
 
   show "typed \<V>' (t \<cdot>t \<rho>) \<tau> \<longleftrightarrow> typed \<V> t \<tau>"
   proof(intro iffI)
     assume "typed \<V>' (t \<cdot>t \<rho>) \<tau>"
-    with renaming  show "typed \<V> t \<tau>"
+    with \<V> show "typed \<V> t \<tau>"
     proof(induction t arbitrary: \<tau>)
       case (Var x)
-      then obtain y where y: "Var x \<cdot>t \<rho> = Var y"
-        by (metis eval_term.simps(1) term.collapse(1) term_subst_is_renaming_iff)
+      
+      have "\<V>' (term.rename \<rho> x) = \<tau>"
+        using Var term.id_subst_rename[OF renaming]
+        by (metis eval_term.simps(1) term.typed.right_uniqueD typed.Var)
 
-      then have "\<V> (inv \<rho> (Var y)) = \<V>' y"
-        by (simp add: Var)
-
-      moreover have "(inv \<rho> (Var y)) = x"
-        using y renaming
-        unfolding term_subst_is_renaming_iff
-        by (metis eval_term.simps(1) inv_f_f)
-
-      moreover have "\<V>' y = \<tau>"
-        using Var
-        unfolding y
-        using typed.Var by fastforce
-
-      ultimately have "\<V> x = \<tau>"
-        by blast
+      then have "\<V> x = \<tau>"
+        by (simp add: renaming Var.prems)
 
       then show ?case
         by(rule typed.Var)
@@ -257,30 +246,16 @@ next
   next
     assume "typed \<V> t \<tau>"
     then show "typed \<V>' (t \<cdot>t \<rho>) \<tau>"
-      using renaming
+      using \<V>
     proof(induction rule: typed.induct)
       case (Var x \<tau>)
 
-      obtain y where y: "Var x \<cdot>t \<rho> = Var y"
-        using renaming
-        by (metis eval_term.simps(1) term.collapse(1) term_subst_is_renaming_iff)
-
-      then have "\<V> (inv \<rho> (Var y)) = \<V>' y"
-        using Var(3)
-        by simp     
-
-      moreover have "(inv \<rho> (Var y)) = x"
-        using y renaming
-        unfolding term_subst_is_renaming_iff
-        by (metis eval_term.simps(1) inv_f_f)
-
-      ultimately have "\<V>' y = \<tau>"
-        using Var
-        by argo
+      have "\<V>' (term.rename \<rho> x) = \<tau>"
+        using Var.hyps Var.prems 
+        by auto
 
       then show ?case
-        unfolding y
-        by(rule typed.Var)
+        by (metis eval_term.simps(1) renaming term.id_subst_rename typed.Var)
     next
       case (Fun f \<tau>s \<tau> ts)
 
@@ -290,11 +265,11 @@ next
   qed
 next
 
-  fix \<V> \<V>' :: "('v, 'ty) var_types" and t :: "('f, 'v) term" and \<rho> \<tau>
+  fix \<V> \<V>' :: "('v, 'ty) var_types" and t :: "('f, 'v) term" and \<rho> :: "('f, 'v) subst" and \<tau>
 
   assume 
     renaming: "term_subst.is_renaming \<rho>" and
-    \<V>: "\<forall>x\<in>term.vars (t \<cdot>t \<rho>). \<V> (inv \<rho> (Var x)) = \<V>' x"
+    \<V>: "\<forall>x\<in>term.vars t. \<V> x = \<V>' (term.rename \<rho> x)"
 
   then show "welltyped \<V>' (t \<cdot>t \<rho>) \<tau> \<longleftrightarrow> welltyped \<V> t \<tau>"
   proof(intro iffI)
@@ -305,24 +280,12 @@ next
     proof(induction t arbitrary: \<tau>)
       case (Var x)
 
-      then obtain y where y: "Var x \<cdot>t \<rho> = Var y"
-        by (metis eval_term.simps(1) renaming term.collapse(1) term_subst_is_renaming_iff)
+      then have "\<V>' (term.rename \<rho> x) = \<tau>"
+        using renaming term.id_subst_rename[OF renaming]
+        by (metis eval_term.simps(1) term.typed.right_uniqueD term.typed_if_welltyped typed.Var)
 
-      then have "\<V> (inv \<rho> (Var y)) = \<V>' y"
-        by (simp add: Var)
-
-      moreover have "(inv \<rho> (Var y)) = x"
-        using y renaming
-        unfolding term_subst_is_renaming_iff
-        by (metis eval_term.simps(1) inv_f_f)
-
-      moreover have "\<V>' y = \<tau>"
-        using Var
-        unfolding y
-        using welltyped.Var by fastforce
-
-      ultimately have "\<V> x = \<tau>"
-        by blast
+      then have "\<V> x = \<tau>"
+        by (simp add: Var.prems(1))
 
       then show ?case
         by(rule welltyped.Var)
@@ -353,25 +316,12 @@ next
     proof(induction rule: welltyped.induct)
       case (Var x \<tau>)
 
-      obtain y where y: "Var x \<cdot>t \<rho> = Var y"
-        using renaming
-        by (metis eval_term.simps(1) term.collapse(1) term_subst_is_renaming_iff)
-
-      then have "\<V> (inv \<rho> (Var y)) = \<V>' y"
-        by (simp add: Var.prems)
-
-      moreover have "(inv \<rho> (Var y)) = x"
-        using y renaming
-        unfolding term_subst_is_renaming_iff
-        by (metis eval_term.simps(1) inv_f_f)
-
-      ultimately have "\<V>' y = \<tau>"
-        using Var
-        by argo
+      then have "\<V>' (term.rename \<rho> x) = \<tau>"
+        by simp
 
       then show ?case
-        unfolding y
-        by(rule welltyped.Var)
+        using term.id_subst_rename[OF renaming]
+        by (metis eval_term.simps(1) welltyped.Var)
     next
       case (Fun f \<tau>s \<tau> ts)
 
