thys/Superposition_Calculus/Superposition.thy
@@ -48,9 +48,8 @@ locale superposition_calculus =
     tiebreakers :: "'f gatom clause \<Rightarrow> ('f, 'v) atom clause \<Rightarrow> ('f, 'v) atom clause \<Rightarrow> bool" 
   assumes
     tiebreakers: "\<And>C\<^sub>G. wellfounded_strict_order (tiebreakers C\<^sub>G)" and
-    (* TODO: Move to locale assumption *)
-    variables: "|UNIV :: 'ty set| \<le>o |UNIV :: 'v set|" and
-    ground_critical_pair_theorem: "\<And>(R :: 'f gterm rel). ground_critical_pair_theorem R"
+    types_ordLeq_variables: "|UNIV :: 'ty set| \<le>o |UNIV :: 'v set|" and
+    ground_critical_pair_theorem: "\<And>R :: 'f gterm rel. ground_critical_pair_theorem R"
 begin
 
 interpretation term_order_notation.
@@ -99,14 +98,13 @@ inductive eq_factoring :: "('f, 'v, 'ty) typed_clause \<Rightarrow> ('f, 'v, 'ty
     C = add_mset (t\<^sub>1 \<approx> t\<^sub>2') (add_mset (t\<^sub>1' !\<approx> t\<^sub>2') D') \<cdot> \<mu> \<Longrightarrow>
     eq_factoring (D, \<V>) (C, \<V>)"
 
-(* TODO: Get things like is_renaming out of the name scope *)
-(* TODO: \<forall>x \<in> clause.vars (D \<cdot> \<rho>\<^sub>2). \<V>\<^sub>2 (inv \<rho>\<^sub>2 (Var x)) = \<V>\<^sub>3 x *)
+(* TODO: infinite_variables_per_type \<V>\<^sub>1 *)
 inductive superposition ::
   "('f, 'v, 'ty) typed_clause \<Rightarrow> ('f, 'v, 'ty) typed_clause \<Rightarrow> ('f, 'v, 'ty) typed_clause \<Rightarrow> bool"
 where
   superpositionI:
-   "term.is_renaming \<rho>\<^sub>1 \<Longrightarrow>
-    term.is_renaming \<rho>\<^sub>2 \<Longrightarrow>
+   "term_subst.is_renaming \<rho>\<^sub>1 \<Longrightarrow>
+    term_subst.is_renaming \<rho>\<^sub>2 \<Longrightarrow>
     clause.vars (E \<cdot> \<rho>\<^sub>1) \<inter> clause.vars (D \<cdot> \<rho>\<^sub>2) = {} \<Longrightarrow>
     E = add_mset l\<^sub>1 E' \<Longrightarrow>
     D = add_mset l\<^sub>2 D' \<Longrightarrow>
@@ -115,8 +113,8 @@ where
     l\<^sub>2 = t\<^sub>2 \<approx> t\<^sub>2' \<Longrightarrow>
     \<not> is_Var t\<^sub>1 \<Longrightarrow>
     welltyped_imgu_on (clause.vars (E \<cdot> \<rho>\<^sub>1) \<union> clause.vars (D \<cdot> \<rho>\<^sub>2)) \<V>\<^sub>3 (t\<^sub>1 \<cdot>t \<rho>\<^sub>1) (t\<^sub>2 \<cdot>t \<rho>\<^sub>2) \<mu> \<Longrightarrow>
-    \<forall>x \<in> clause.vars (E \<cdot> \<rho>\<^sub>1). \<V>\<^sub>1 (inv \<rho>\<^sub>1 (Var x)) = \<V>\<^sub>3 x \<Longrightarrow>
-    \<forall>x \<in> clause.vars (D \<cdot> \<rho>\<^sub>2). \<V>\<^sub>2 (inv \<rho>\<^sub>2 (Var x)) = \<V>\<^sub>3 x \<Longrightarrow>
+    \<forall>x \<in> clause.vars E. \<V>\<^sub>1 x = \<V>\<^sub>3 (term.rename \<rho>\<^sub>1 x) \<Longrightarrow>
+    \<forall>x \<in> clause.vars D. \<V>\<^sub>2 x = \<V>\<^sub>3 (term.rename \<rho>\<^sub>2 x) \<Longrightarrow>
     is_welltyped_on (clause.vars E) \<V>\<^sub>1 \<rho>\<^sub>1 \<Longrightarrow>
     is_welltyped_on (clause.vars D) \<V>\<^sub>2 \<rho>\<^sub>2 \<Longrightarrow>
     (\<And>\<tau> \<tau>'. typed \<V>\<^sub>2 t\<^sub>2 \<tau> \<Longrightarrow> typed \<V>\<^sub>2 t\<^sub>2' \<tau>' \<Longrightarrow> \<tau> = \<tau>') \<Longrightarrow>
@@ -125,7 +123,7 @@ where
       \<and> select E = {#} 
       \<and> is_strictly_maximal (l\<^sub>1 \<cdot>l \<rho>\<^sub>1 \<odot> \<mu>) (E \<cdot> \<rho>\<^sub>1 \<odot> \<mu>)) \<or>
     (\<P> = Neg 
-      \<and> (select E = {#} \<and> is_maximal (l\<^sub>1 \<cdot>l \<rho>\<^sub>1 \<odot> \<mu>) (E \<cdot> \<rho>\<^sub>1 \<odot> \<mu>) 
+      \<and> (select E = {#} \<and> is_maximal (l\<^sub>1 \<cdot>l \<rho>\<^sub>1 \<odot> \<mu>) (E \<cdot> \<rho>\<^sub>1 \<odot> \<mu>)
           \<or> is_maximal (l\<^sub>1 \<cdot>l \<rho>\<^sub>1 \<odot> \<mu>) ((select E) \<cdot> \<rho>\<^sub>1 \<odot> \<mu>))) \<Longrightarrow>
     select D = {#} \<Longrightarrow>
     is_strictly_maximal (l\<^sub>2 \<cdot>l \<rho>\<^sub>2 \<odot> \<mu>) (D \<cdot> \<rho>\<^sub>2 \<odot> \<mu>) \<Longrightarrow>
@@ -156,9 +154,9 @@ subsubsection \<open>Alternative Specification of the Superposition Rule\<close>
 inductive pos_superposition ::
   "('f, 'v, 'ty) typed_clause \<Rightarrow> ('f, 'v, 'ty) typed_clause \<Rightarrow> ('f, 'v, 'ty) typed_clause \<Rightarrow> bool"
 where
-  pos_superpositionI: "
-    term.is_renaming \<rho>\<^sub>1 \<Longrightarrow>
-    term.is_renaming \<rho>\<^sub>2 \<Longrightarrow>
+  pos_superpositionI: 
+   "term_subst.is_renaming \<rho>\<^sub>1 \<Longrightarrow>
+    term_subst.is_renaming \<rho>\<^sub>2 \<Longrightarrow>
     clause.vars (E \<cdot> \<rho>\<^sub>1) \<inter> clause.vars (D \<cdot> \<rho>\<^sub>2) = {} \<Longrightarrow>
     E = add_mset l\<^sub>1 E' \<Longrightarrow>
     D = add_mset l\<^sub>2 D' \<Longrightarrow>
@@ -166,8 +164,8 @@ where
     l\<^sub>2 = t\<^sub>2 \<approx> t\<^sub>2' \<Longrightarrow>
     \<not> is_Var t\<^sub>1 \<Longrightarrow>
     welltyped_imgu_on (clause.vars (E \<cdot> \<rho>\<^sub>1) \<union> clause.vars (D \<cdot> \<rho>\<^sub>2)) \<V>\<^sub>3 (t\<^sub>1 \<cdot>t \<rho>\<^sub>1) (t\<^sub>2 \<cdot>t \<rho>\<^sub>2) \<mu> \<Longrightarrow>
-    \<forall>x \<in> clause.vars (E \<cdot> \<rho>\<^sub>1). \<V>\<^sub>1 (inv \<rho>\<^sub>1 (Var x)) = \<V>\<^sub>3 x \<Longrightarrow>
-    \<forall>x \<in> clause.vars (D \<cdot> \<rho>\<^sub>2). \<V>\<^sub>2 (inv \<rho>\<^sub>2 (Var x)) = \<V>\<^sub>3 x \<Longrightarrow>
+    \<forall>x \<in> clause.vars E. \<V>\<^sub>1 x = \<V>\<^sub>3 (term.rename \<rho>\<^sub>1 x) \<Longrightarrow>
+    \<forall>x \<in> clause.vars D. \<V>\<^sub>2 x = \<V>\<^sub>3 (term.rename \<rho>\<^sub>2 x) \<Longrightarrow>
     is_welltyped_on (clause.vars E) \<V>\<^sub>1 \<rho>\<^sub>1 \<Longrightarrow>
     is_welltyped_on (clause.vars D) \<V>\<^sub>2 \<rho>\<^sub>2 \<Longrightarrow>
     (\<And>\<tau> \<tau>'. typed \<V>\<^sub>2 t\<^sub>2 \<tau> \<Longrightarrow> typed \<V>\<^sub>2 t\<^sub>2' \<tau>' \<Longrightarrow> \<tau> = \<tau>') \<Longrightarrow>
@@ -198,8 +196,8 @@ inductive neg_superposition ::
   "('f, 'v, 'ty) typed_clause \<Rightarrow> ('f, 'v, 'ty) typed_clause \<Rightarrow> ('f, 'v, 'ty) typed_clause \<Rightarrow> bool"
 where
   neg_superpositionI: "
-    term.is_renaming \<rho>\<^sub>1 \<Longrightarrow>
-    term.is_renaming \<rho>\<^sub>2 \<Longrightarrow>
+    term_subst.is_renaming \<rho>\<^sub>1 \<Longrightarrow>
+    term_subst.is_renaming \<rho>\<^sub>2 \<Longrightarrow>
     clause.vars (E \<cdot> \<rho>\<^sub>1) \<inter> clause.vars (D \<cdot> \<rho>\<^sub>2) = {} \<Longrightarrow>
     E = add_mset l\<^sub>1 E' \<Longrightarrow>
     D = add_mset l\<^sub>2 D' \<Longrightarrow>
@@ -207,8 +205,8 @@ where
     l\<^sub>2 = t\<^sub>2 \<approx> t\<^sub>2' \<Longrightarrow>
     \<not> is_Var t\<^sub>1 \<Longrightarrow>
     welltyped_imgu_on (clause.vars (E \<cdot> \<rho>\<^sub>1) \<union> clause.vars (D \<cdot> \<rho>\<^sub>2)) \<V>\<^sub>3 (t\<^sub>1 \<cdot>t \<rho>\<^sub>1) (t\<^sub>2 \<cdot>t \<rho>\<^sub>2) \<mu> \<Longrightarrow>
-    \<forall>x \<in> clause.vars (E \<cdot> \<rho>\<^sub>1). \<V>\<^sub>1 (inv \<rho>\<^sub>1 (Var x)) = \<V>\<^sub>3 x \<Longrightarrow>
-    \<forall>x \<in> clause.vars (D \<cdot> \<rho>\<^sub>2). \<V>\<^sub>2 (inv \<rho>\<^sub>2 (Var x)) = \<V>\<^sub>3 x \<Longrightarrow>
+    \<forall>x \<in> clause.vars E. \<V>\<^sub>1 x = \<V>\<^sub>3 (term.rename \<rho>\<^sub>1 x) \<Longrightarrow>
+    \<forall>x \<in> clause.vars D. \<V>\<^sub>2 x = \<V>\<^sub>3 (term.rename \<rho>\<^sub>2 x) \<Longrightarrow>
     is_welltyped_on (clause.vars E) \<V>\<^sub>1 \<rho>\<^sub>1 \<Longrightarrow>
     is_welltyped_on (clause.vars D) \<V>\<^sub>2 \<rho>\<^sub>2 \<Longrightarrow>
     (\<And>\<tau> \<tau>'. typed \<V>\<^sub>2 t\<^sub>2 \<tau> \<Longrightarrow> typed \<V>\<^sub>2 t\<^sub>2' \<tau>' \<Longrightarrow> \<tau> = \<tau>') \<Longrightarrow>
